keccak: definition with less monadic operations

Garden/Plonky3/keccak/round_flags.v
@@ -25,43 +25,42 @@ pub(crate) fn eval_round_flags<AB: AirBuilder>(builder: &mut AB) {
         }));
 }
 *)
-Definition eval_round_flags (is_first_row is_transition : bool) (local next : KeccakCols.t) :
+Definition eval_round_flags {p} `{Prime p}
+    (is_first_row is_transition : bool)
+    (local next : KeccakCols.t) :
     M.t unit :=
-  let* _ := when is_first_row [[
-    assert_one (| Array.get (| local.(KeccakCols.step_flags), 0 |) |)
-  ]] in
-  let* _ := when is_first_row [[
-    assert_zeros (| Array.slice_from local.(KeccakCols.step_flags) 1 |)
-  ]] in
-  let* _ := when is_transition [[
-    assert_zeros (N := NUM_ROUNDS) (| Array.from_fn (| fun i => [[
-      M.sub (|
-        Array.get (| local.(KeccakCols.step_flags), i |),
-        Array.get (| next.(KeccakCols.step_flags), (i + 1) mod NUM_ROUNDS |)
-      |)
-    ]] |) |)
-  ]] in
-  M.Pure tt.
+  let* _ := when is_first_row (
+    M.equal (local.(KeccakCols.step_flags).(Array.get) 0) 1
+  ) in
+  let* _ := when is_first_row (
+    M.zeros (Array.slice_from local.(KeccakCols.step_flags) 1)
+  ) in
+  let* _ := when is_transition (
+    M.zeros (N := NUM_ROUNDS) {|
+      Array.get i :=
+        BinOp.sub (local.(KeccakCols.step_flags).(Array.get) i)
+        (next.(KeccakCols.step_flags).(Array.get) ((i + 1) mod NUM_ROUNDS))
+    |}
+  ) in
+  M.pure tt.
 
-Definition eval_round_flags_step_flags
+(* Definition eval_round_flags_step_flags {p} `{Prime p}
     (is_first_row is_transition : bool)
     (local next : Array.t Z NUM_ROUNDS) :
     M.t unit :=
-  let* _ := when is_first_row [[
-    assert_one (| Array.get (| local, 0 |) |)
-  ]] in
-  let* _ := when is_first_row [[
-    assert_zeros (| Array.slice_from local 1 |)
-  ]] in
-  let* _ := when is_transition [[
-    assert_zeros (N := NUM_ROUNDS) (| Array.from_fn (| fun i => [[
-      M.sub (|
-        Array.get (| local, i |),
-        Array.get (| next, (i + 1) mod NUM_ROUNDS |)
-      |)
-    ]] |) |)
-  ]] in
-  M.Pure tt.
+  let* _ := when is_first_row (
+    assert_one (local.(Array.get) 0)
+  ) in
+  let* _ := when is_first_row (
+      M.zeros (Array.slice_from local 1)
+  ) in
+  let* _ := when is_transition (
+    M.zeros (N := NUM_ROUNDS) {|
+      Array.get i :=
+        BinOp.sub (local.(Array.get) i) (next.(Array.get) ((i + 1) mod NUM_ROUNDS))
+    |}
+  ) in
+  M.pure tt. *)
 
 (* Definition eval_round_flags_explicit
     (is_first_row is_transition : bool)
@@ -84,130 +83,59 @@ Definition eval_round_flags_step_flags
   M.Pure tt. *)
 
 Module Spec.
-  Lemma spec_first_row (p : Z)
-      (local next : StepFlagsInput.t)
-      (H_p : IsPrime p) :
-    {{ M.eval p (eval_round_flags_step_flags true false
-        (StepFlagsInput.to_value local) (StepFlagsInput.to_value next)) 🔽
+  Lemma spec_first_row {p} `{Prime p}
+      (local next : KeccakCols.t) :
+    {{ eval_round_flags true false local next 🔽
       tt,
-      StepFlagsInput.to_value local = StepFlagsOutput.to_value 0
+      forall i, 0 <= i < NUM_ROUNDS ->
+      local.(KeccakCols.step_flags).(Array.get) i =
+      if i =? 0 then 1 else 0
     }}.
   Proof.
-    destruct local.
-    cbn; unfold Pos.to_nat; cbn.
-    eapply Run.Equiv. {
+    eapply Run.Implies. {
       progress repeat (
         apply Run.Pure ||
         eapply Run.Let ||
-        apply Run.Equal
+        apply Run.Equal ||
+        apply Run.Zeros ||
+        cbn
       ).
     }
-    unfold StepFlagsInput.to_value, StepFlagsOutput.to_value, Array.from_fn_pure; cbn.
-    unfold Pos.to_nat; cbn.
-    split; sauto lq: on rew: off.
+    with_strategy opaque [Z.add] cbn.
+    intros.
+    destruct (i =? 0) eqn:H_eq; try lia.
+    {
+      assert (i = 0) by lia.
+      sfirstorder.
+    }
+    { assert (1 <= i < NUM_ROUNDS) by lia.
+      intuition.
+      match goal with
+      | [ H : _ |- _ ] =>
+        rewrite <- (H (i - 1)) by lia
+      end.
+      f_equal; lia.
+    }
   Qed.
 
-  Lemma spec_transition (p : Z)
-      (local : StepFlagsOutput.t)
-      (next : StepFlagsInput.t)
-      (H_p : IsPrime p) :
-    {{ M.eval p (eval_round_flags_step_flags false true
-        (StepFlagsOutput.to_value local) (StepFlagsInput.to_value next)) 🔽
+  Lemma spec_transition {p} `{Prime p}
+      (local next : KeccakCols.t) :
+    {{ eval_round_flags false true local next 🔽
       tt,
-      StepFlagsInput.to_value next = StepFlagsOutput.to_value (local + 1)
+      forall i, 0 <= i < NUM_ROUNDS ->
+      local.(KeccakCols.step_flags).(Array.get) i =
+      next.(KeccakCols.step_flags).(Array.get) ((i + 1) mod NUM_ROUNDS)
     }}.
   Proof.
-    (* destruct next. *)
-    (* unfold StepFlagsOutput.to_value, Array.from_fn_pure; cbn.
-    unfold Pos.to_nat, Array.get; cbn. *)
-    eapply Run.Equiv; cbn. {
+    eapply Run.Implies. {
       progress repeat (
         apply Run.Pure ||
         eapply Run.Let ||
-        apply Run.Equal
+        apply Run.Equal ||
+        apply Run.AssertZerosFromFnSub ||
+        cbn
       ).
     }
-    replace local with 15 by admit.
-    cbn.
-    withcbn.
-    split; sauto lq: on rew: off.
-
-  Definition initial_step_flags : Array.t Z NUM_ROUNDS :=
-    Array.from_fn_pure (fun i =>
-      if i =? 0 then 1 else 0
-    ).
-
-  Definition initial_step_flags_explicit : ExplicitArray.t Z NUM_ROUNDS :=
-    ExplicitArray.from_fn (length := NUM_ROUNDS) (fun i =>
-      if i =? 0 then 1 else 0
-    ).
-
-  Definition shift (local_step_flags next_step_flags : Array.t Z NUM_ROUNDS) : Prop :=
-    forall i,
-      Array.get local_step_flags i =
-      Array.get next_step_flags ((i + 1) mod NUM_ROUNDS).
-
-  Definition spec (is_first_row is_transition : bool) (local next : KeccakCols.t) : Prop :=
-    if is_first_row then
-      local.(KeccakCols.step_flags) = initial_step_flags
-    else if is_transition then
-      shift local.(KeccakCols.step_flags) next.(KeccakCols.step_flags)
-    else
-      True.
-
-  Definition spec_step_flags (is_first_row is_transition : bool) (local next : Array.t Z NUM_ROUNDS) : Prop :=
-    if is_first_row then
-      local = initial_step_flags
-    else if is_transition then
-      shift local next
-    else
-      True.
-
-  Definition spec_step_flags_explicit (is_first_row is_transition : bool) (local next : ExplicitArray.t Z NUM_ROUNDS) : Prop :=
-    if is_first_row then
-      local = initial_step_flags_explicit
-    else if is_transition then
-      shift (ExplicitArray.to_array local) (ExplicitArray.to_array next)
-    else
-      True.
-
-  (* Notation "array [< >]" := (array.(Pair.x)) (at level 100).
-  Notation "array [< .. >]" := (array.(Pair.xs)) (at level 100). *)
-
-  Lemma spec_correct_step_flags (p : Z)
-    (local next : ExplicitArray.t Z NUM_ROUNDS)
-    (H_p : IsPrime p) :
-    let local_array := ExplicitArray.to_array local in
-    let next_array := ExplicitArray.to_array next in
-    {{ M.eval p (eval_round_flags_step_flags true false local_array next_array) 🔽
-      tt, spec_step_flags_explicit true false local next
-    }}.
-  Proof.
-    do 24 destruct local as [? local].
-    cbn; unfold Pos.to_nat; cbn.
-    eapply Run.Equiv. {
-      progress repeat (
-        apply Run.Pure ||
-        eapply Run.Let ||
-        apply Run.Equal
-      ).
-    }
-    split; sauto lq: on rew: off.
+    easy.
   Qed.
-
-  Lemma spec_correct (p : Z) (is_first_row is_transition : bool) (local next : KeccakCols.t)
-    (H_p : IsPrime p)
-    (H_local : KeccakCols.Valid.t local)
-    (H_next : KeccakCols.Valid.t next) :
-    {{ M.eval p (eval_round_flags is_first_row is_transition local next) 🔽
-      tt, spec is_first_row is_transition local next
-    }}.
-  Proof.
-    destruct H_local, H_next.
-    (* Print Array.Valid.t.
-    destruct is_first_row, is_transition; cbn.
-    { eapply Run.Equiv. {
-        destruct local.(KeccakCols.step_flags).(Array.value).
-      }
-
-    } *)
+End Spec.
